Repair flatProps, distractions improving proofs
Whether it's really an improvement is questionable, but the
additional level of transitivity needed in some of the new
evaluate proofs was pretty bad, so it was worth trying to do
something.

compiler/backend/semantics/flatPropsScript.sml
@@ -281,7 +281,7 @@ Theorem evaluate_length:
 Proof
   ho_match_mp_tac (evaluate_ind |> Q.SPECL [`P`, `\_ _. T`, `\_ _. T`]
     |> SIMP_RULE bool_ss [] |> Q.GEN `P`) >>
-  srw_tac[][evaluate_def] >> srw_tac[][] >>
+  srw_tac[][evaluate_def, LET_DEF] >> srw_tac[][] >>
   every_case_tac >> full_simp_tac(srw_ss())[] >> srw_tac[][]
 QED
 
@@ -328,7 +328,7 @@ QED
 
 Theorem do_app_state_unchanged:
   !c s op vs s' r. do_app s op vs = SOME (s', r) ⇒
-     s'.c = s.c ∧ s'.eval_mode = s.eval_mode
+     s'.c = s.c ∧ s'.eval_mode = s.eval_mode ∧ s'.clock = s.clock
 Proof
   rw [do_app_cases] >>
   fs [semanticPrimitivesTheory.store_assign_def] >>
@@ -362,81 +362,29 @@ Proof
   metis_tac [PAIR_EQ]
 QED
 
-val do_app_add_to_clock = Q.prove (
-  `do_app ^s op es = SOME (t, r)
-   ==>
-   do_app (s with clock := s.clock + k) op es =
-     SOME (t with clock := t.clock + k, r)`,
-  rw [do_app_cases] \\ fs []);
-
-val do_app_add_to_clock_NONE = Q.prove (
-  `do_app ^s op es = NONE
-   ==>
-   do_app (s with clock := s.clock + k) op es = NONE`,
-  Cases_on `op` \\ rw [do_app_def]
-  \\ fs [case_eq_thms, pair_case_eq] \\ rw [] \\ fs []
-  \\ rpt (pairarg_tac \\ fs [])
-  \\ fs [bool_case_eq, case_eq_thms]
-  \\ fs [IS_SOME_EXISTS,CaseEq"option",CaseEq"store_v"]);
-
-Theorem do_eval_clock_change:
-  do_eval vs (s with clock updated_by f) = (case do_eval vs s of
-      NONE => NONE
-    | SOME (r, s', v) => SOME (r, (s' with clock updated_by f), v))
+Triviality do_app_clock_change:
+  do_app ((^s) with clock := clk) op es =
+     (case do_app s op es of NONE => NONE
+        | SOME (t, r) => SOME (t with clock := clk, r))
 Proof
-  TOP_CASE_TAC
-  \\ fs [do_eval_def, CaseEq "eval_config", list_case_eq, option_case_eq]
-  \\ rpt (pairarg_tac \\ fs [])
-  \\ fs [option_case_eq, pair_case_eq]
-  \\ rveq \\ fs []
-QED
-
-val do_eval_add_to_clock = REWRITE_RULE
-    [ASSUME ``do_eval vs s = SOME (r, t, v)``] do_eval_clock_change
-  |> DISCH_ALL
-
-val do_eval_add_to_clock_NONE = REWRITE_RULE
-    [ASSUME ``do_eval vs s = NONE``] do_eval_clock_change
-  |> DISCH_ALL
-
-Theorem evaluate_add_to_clock:
-   (∀env ^s es s' r.
-       evaluate env s es = (s',r) ∧
-       r ≠ Rerr (Rabort Rtimeout_error) ⇒
-       evaluate env (s with clock := s.clock + extra) es =
-         (s' with clock := s'.clock + extra,r)) ∧
-   (∀^s d s' r.
-       evaluate_dec s d = (s',r) ∧
-       r ≠ SOME (Rabort Rtimeout_error) ⇒
-       evaluate_dec (s with clock := s.clock + extra) d =
-         (s' with clock := s'.clock + extra,r)) ∧
-   (∀^s ds s' r.
-       evaluate_decs s ds = (s',r) ∧
-       r ≠ SOME (Rabort Rtimeout_error) ⇒
-       evaluate_decs (s with clock := s.clock + extra) ds =
-         (s' with clock := s'.clock + extra,r))
-Proof
-  ho_match_mp_tac evaluate_ind \\ rw [evaluate_def]
-  \\ fs [case_eq_thms, pair_case_eq] \\ rw [] \\ fs [PULL_EXISTS]
-  \\ rw [] \\ fs [pmatch_ignore_clock]
-  \\ fs [case_eq_thms, pair_case_eq, bool_case_eq, CaseEq"match_result"] \\ rw []
-  \\ fs [dec_clock_def]
-  \\ fs [do_eval_clock_change]
-  \\ map_every imp_res_tac
-      [do_app_add_to_clock_NONE,
-       do_app_add_to_clock,
-       do_eval_clock] \\ fs []
-  \\ every_case_tac \\ fs []
-QED
-
-Theorem evaluate_decs_add_to_clock:
-  ∀decs s s' r.
-   r ≠ SOME (Rabort Rtimeout_error) ∧
-   evaluate_decs s decs = (s',r) ⇒
-   evaluate_decs (s with clock := s.clock + extra) decs =
-   (s' with clock := s'.clock + extra,r)
-Proof
-  metis_tac [evaluate_add_to_clock]
+  reverse CASE_TAC
+  >- (
+    Cases_on `x`
+    \\ pop_assum (assume_tac o REWRITE_RULE [do_app_cases])
+    \\ fs [] \\ rveq \\ fs []
+    \\ rveq \\ fs []
+    \\ rfs []
+    \\ simp [do_app_def]
+  )
+  >- (
+    Cases_on `op`
+    \\ pop_assum (mp_tac o REWRITE_RULE [do_app_def]) \\ rw []
+    \\ fs [case_eq_thms, pair_case_eq] \\ rw [] \\ fs []
+    \\ rpt (pairarg_tac \\ fs [])
+    \\ fs [do_app_def, bool_case_eq, case_eq_thms]
+    \\ rw []
+    \\ fs [IS_SOME_EXISTS,CaseEq"option",CaseEq"store_v"]
+  )
 QED
 
 Theorem do_app_io_events_mono:
@@ -453,71 +401,96 @@ Proof
 QED
 
 Theorem evaluate_io_events_mono:
-   (∀env ^s es.
-      s.ffi.io_events ≼ (FST (evaluate env s es)).ffi.io_events) ∧
-   (∀^s d.
-      s.ffi.io_events ≼ (FST (evaluate_dec s d)).ffi.io_events) ∧
-   (∀^s ds.
-      s.ffi.io_events ≼ (FST (evaluate_decs s ds)).ffi.io_events)
+   (∀env ^s es s' r.
+      evaluate env s es = (s', r) ==>
+      s.ffi.io_events ≼ s'.ffi.io_events) ∧
+   (∀^s d s' r.
+      evaluate_dec s d = (s', r) ==>
+      s.ffi.io_events ≼ s'.ffi.io_events) ∧
+   (∀^s ds s' r.
+      evaluate_decs s ds = (s', r) ==>
+      s.ffi.io_events ≼ s'.ffi.io_events)
 Proof
   ho_match_mp_tac evaluate_ind \\ rw [evaluate_def]
   \\ every_case_tac \\ fs [] \\ rfs []
+  \\ rveq \\ fs []
   \\ fs [dec_clock_def]
   \\ imp_res_tac do_app_io_events_mono \\ fs []
-  \\ imp_res_tac do_eval_clock \\ fs []
+  \\ fsrw_tac [SATISFY_ss] [IS_PREFIX_TRANS]
   \\ metis_tac [IS_PREFIX_TRANS]
 QED
 
-Theorem with_clock_ffi:
-   (s with clock := k).ffi = s.ffi
+(* captures the relationship between two evaluate results for different
+   clock amounts *)
+Definition clock_io_mono_res_rel_def:
+  clock_io_mono_res_rel timeout ex res1 res2 = (case (res1, res2) of
+        ((s1, r1), (s2, r2)) =>
+        s1.ffi.io_events ≼ s2.ffi.io_events /\
+        (r1 <> timeout ==> r2 = r1 /\ s2 = (s1 with clock := ex + s1.clock)))
+End
+
+(* complicated looking theorem organises a case split on timeouts, makes
+   some of the transitivity reasoning implicit, and reduces the number of
+   cases in the evaluate proof *)
+Theorem clock_io_mono_res_rel_split:
+    !pre_timeout.
+    (clock_io_mono_res_rel pre_timeout ex res1 res2) /\
+    (! r s1 s2. res1 = (s1, pre_timeout) /\ res2 = (s2, r) ==>
+        (case g1 s1 pre_timeout of (s_fin, r_fin) =>
+            s_fin = s1 /\ r_fin = timeout) /\
+        (case g2 s2 r of (s3, _) => s2.ffi.io_events ≼ s3.ffi.io_events)) /\
+    (! r s. res1 = (s, r) /\
+        res2 = (s with clock := ex + s.clock, r) /\
+        r <> pre_timeout ==>
+        clock_io_mono_res_rel timeout ex (g1 s r)
+            (g2 (s with clock := ex + s.clock) r)) ==>
+    clock_io_mono_res_rel timeout ex
+        (pair_CASE res1 g1) (pair_CASE res2 g2)
 Proof
-  EVAL_TAC
+  rw [clock_io_mono_res_rel_def]
+  \\ every_case_tac
+  \\ fs []
+  \\ imp_res_tac IMP_DISJ_THM
+  \\ fs [] \\ rfs []
+  \\ rveq \\ fs []
+  \\ fsrw_tac [SATISFY_ss] [IS_PREFIX_TRANS]
 QED
 
-Theorem evaluate_add_to_clock_io_events_mono:
-   (∀env ^s es extra.
-       (FST (evaluate env s es)).ffi.io_events ≼
-       (FST (evaluate env (s with clock := s.clock + extra) es)).ffi.io_events)
-   ∧
-   (∀^s d extra.
-       (FST (evaluate_dec s d)).ffi.io_events ≼
-       (FST (evaluate_dec (s with clock := s.clock + extra) d)).ffi.io_events) ∧
-   (∀^s ds extra.
-       (FST (evaluate_decs s ds)).ffi.io_events ≼
-       (FST (evaluate_decs (s with clock := s.clock + extra) ds)).ffi.io_events)
-Proof
-  ho_match_mp_tac evaluate_ind \\ rw [evaluate_def] \\ fs []
-  \\ rpt (PURE_FULL_CASE_TAC \\ fs []) \\ rfs []
-  \\ map_every imp_res_tac [evaluate_add_to_clock,
-                            evaluate_io_events_mono,
-                            do_app_add_to_clock_NONE,
-                            do_app_add_to_clock,
-                            do_eval_add_to_clock_NONE,
-                            do_eval_add_to_clock,
-                            do_eval_clock]
-  \\ fs [dec_clock_def, pmatch_ignore_clock]
-  \\ rw [] \\ fs [] \\ rw [] \\ fs []
-  \\ imp_res_tac do_eval_clock \\ rfs []
-  \\ metis_tac [IS_PREFIX_TRANS, FST, PAIR,
-                evaluate_io_events_mono,
-                with_clock_ffi,
-                do_app_io_events_mono]
-QED
+Overload io_mono1[local] =
+  ``clock_io_mono_res_rel (Rerr (Rabort Rtimeout_error))``
+Overload io_mono2[local] =
+  ``clock_io_mono_res_rel (SOME (Rabort Rtimeout_error))``
 
-Theorem evaluate_dec_io_events_mono:
-  ∀z y.
-     y.ffi.io_events ≼ (FST (evaluate_dec y z)).ffi.io_events
-Proof
-  Cases \\ rw [evaluate_def] \\ every_case_tac \\ fs [] \\ rw []
-  \\ metis_tac [evaluate_io_events_mono, FST]
-QED;
+Triviality io_mono_split1 = Q.ISPEC
+  `Rerr (Rabort Rtimeout_error) : ('x, 'y) result`
+  clock_io_mono_res_rel_split
+Triviality io_mono_split2 = Q.ISPEC
+  `SOME (Rabort Rtimeout_error) : 'x error_result option`
+  clock_io_mono_res_rel_split
+Triviality io_mono_tup = clock_io_mono_res_rel_def
+    |> SPEC_ALL |> Q.INST [`res2` |-> `(s2, r)`]
 
-Theorem evaluate_dec_add_to_clock_io_events_mono:
-  ∀prog ^s extra.
-   (FST (evaluate_dec s prog)).ffi.io_events ≼
-   (FST (evaluate_dec (s with clock := s.clock + extra) prog)).ffi.io_events
+Theorem evaluate_clock_io_mono_rel:
+   (∀env ^s es. io_mono1 ex (evaluate env s es)
+        (evaluate env (s with clock := ex + s.clock) es)) ∧
+   (∀ ^s d. io_mono2 ex (evaluate_dec s d)
+        (evaluate_dec (s with clock := ex + s.clock) d)) ∧
+   (∀ ^s ds. io_mono2 ex (evaluate_decs s ds)
+        (evaluate_decs (s with clock := ex + s.clock) ds))
 Proof
-  metis_tac [evaluate_add_to_clock_io_events_mono]
+  ho_match_mp_tac evaluate_ind \\ rw [evaluate_def, LET_DEF]
+  \\ rpt (FIRST [irule io_mono_split1, irule io_mono_split2,
+    CHANGED_TAC (rw [io_mono_tup]), TOP_CASE_TAC])
+  \\ fs [case_eq_thms, pair_case_eq, bool_case_eq, CaseEq"match_result",
+    Q.ISPEC `(a, b)` EQ_SYM_EQ, do_app_clock_change]
+  \\ rveq \\ fs []
+  \\ fs [clock_io_mono_res_rel_def, dec_clock_def]
+  \\ rpt TOP_CASE_TAC
+  \\ imp_res_tac evaluate_io_events_mono
+  \\ imp_res_tac do_app_io_events_mono
+  \\ imp_res_tac do_app_state_unchanged
+  \\ rveq \\ fs []
+  \\ fsrw_tac [SATISFY_ss] [IS_PREFIX_TRANS]
 QED
 
 Theorem evaluate_decs_io_events_mono:
@@ -529,13 +502,15 @@ Proof
   \\ fs []
 QED
 
-Theorem evaluate_decs_add_to_clock_io_events_mono:
-   ∀ds ^s extra.
-     (FST (evaluate_decs s ds)).ffi.io_events ≼
-     (FST (evaluate_decs (s with clock := s.clock + extra) ds)).ffi.io_events
+Theorem evaluate_decs_add_to_clock_io_events_mono_alt:
+    evaluate_decs ^s ds = (s1,res) /\
+    evaluate_decs (s with clock := s.clock + extra) ds = (s2,res2) ==>
+    s1.ffi.io_events ≼ s2.ffi.io_events
 Proof
-  metis_tac [evaluate_add_to_clock_io_events_mono]
-QED;
+  assume_tac (List.last (BODY_CONJUNCTS evaluate_clock_io_mono_rel)
+    |> Q.INST [`ex` |-> `extra`])
+  \\ rw [] \\ fs [clock_io_mono_res_rel_def]
+QED
 
 Theorem evaluate_MAP_Var_local:
   MAP (ALOOKUP env.v) xs = MAP SOME vs ⇒
@@ -647,24 +622,35 @@ Proof
   \\ rw[Once pmatch_nil]
 QED
 
-val evaluate_decs_add_to_clock_initial_state = Q.prove(
-  `r ≠ SOME (Rabort Rtimeout_error) ∧
-   evaluate_decs (initial_state ffi k ec) decs = (s',r) ⇒
-   evaluate_decs (initial_state ffi (ck + k) ec) decs =
-   (s' with clock := s'.clock + ck,r)`,
-  rw [initial_state_def]
-  \\ imp_res_tac evaluate_decs_add_to_clock \\ fs []);
-
-val evaluate_decs_add_to_clock_initial_state_io_events_mono = Q.prove (
-  `evaluate_decs (initial_state ffi k ec) prog = (s',r) ==>
-   s'.ffi.io_events ≼
-   (FST (evaluate_decs (initial_state ffi (k+ck) ec) prog)).ffi.io_events`,
-  rw [initial_state_def]
-  \\ qmatch_assum_abbrev_tac `evaluate_decs s1 _ = _`
-  \\ qispl_then
-         [`prog`,`s1`,`ck`] mp_tac
-         (evaluate_decs_add_to_clock_io_events_mono)
-  \\ fs [Abbr`s1`]);
+Triviality evaluate_decs_initial_state_clocks:
+  evaluate_decs (initial_state ffi k1 ec) decs = (s1, r1) ==>
+  evaluate_decs (initial_state ffi k2 ec) decs = (s2, r2) ==>
+  (k1 = k2 /\ s1 = s2 /\ r1 = r2
+    \/ r1 = SOME (Rabort Rtimeout_error) /\ k1 < k2 /\
+        s1.ffi.io_events ≼ s2.ffi.io_events
+    \/ r2 = SOME (Rabort Rtimeout_error) /\ k2 < k1 /\
+        s2.ffi.io_events ≼ s1.ffi.io_events
+    \/ r1 <> SOME (Rabort Rtimeout_error) /\ r1 = r2 /\
+        ((?k3. k2 = k1 + k3 /\ s2 = s1 with clock := s1.clock + k3)
+            \/ (?k3. k1 = k2 + k3 /\ s1 = s2 with clock := s2.clock + k3)))
+Proof
+  rw []
+  \\ Cases_on `k1 = k2` \\ fs []
+  \\ qspecl_then
+    [`if k1 < k2 then k2 - k1 else k1 - k2`,
+        `initial_state ffi (if k1 < k2 then k1 else k2) ec`, `decs`]
+    mp_tac (List.last (CONJUNCTS evaluate_clock_io_mono_rel) |> GEN_ALL)
+  \\ CASE_TAC
+  \\ fs [clock_io_mono_res_rel_def, initial_state_def]
+  \\ rw []
+  \\ imp_res_tac IMP_DISJ_THM \\ fs []
+  \\ rfs []
+  \\ rveq \\ fs []
+  \\ Cases_on `r1 = SOME (Rabort Rtimeout_error)`
+  \\ simp []
+  \\ TRY (qexists_tac `k2 - k1` \\ simp [] \\ NO_TAC)
+  \\ TRY (qexists_tac `k1 - k2` \\ simp [] \\ NO_TAC)
+QED
 
 val initial_state_with_clock = Q.prove (
   `(initial_state ffi k ec with clock := (initial_state ffi k ec).clock + ck) =
@@ -715,14 +701,10 @@ Proof
       \\ first_x_assum drule
       \\ impl_tac >- (strip_tac \\ fs[])
       \\ strip_tac
-      \\ imp_res_tac evaluate_decs_add_to_clock_initial_state
-      \\ fs[]
-      \\ first_x_assum(qspec_then`ck+k`mp_tac)
-      \\ simp[]
-      \\ Cases_on`res2` \\ Cases_on`r` \\ fs[]
-      \\ TRY(rpt(first_x_assum(qspec_then`k'`mp_tac)) \\ simp[] \\ NO_TAC)
-      \\ every_case_tac \\ fs[] \\ rveq \\ fs[]
-      \\ TRY(rpt(first_x_assum(qspec_then`k'`mp_tac)) \\ simp[] \\ NO_TAC))
+      \\ every_case_tac \\ fs [] \\ rveq \\ fs []
+      \\ dxrule_then drule evaluate_decs_initial_state_clocks
+      \\ simp []
+    )
     \\ DEEP_INTRO_TAC some_intro \\ fs []
     \\ conj_tac
     >- (
@@ -731,16 +713,10 @@ Proof
       \\ first_x_assum drule
       \\ impl_tac >- (strip_tac \\ fs[])
       \\ strip_tac
-      \\ imp_res_tac evaluate_decs_add_to_clock_initial_state
-      \\ fs[]
-      \\ first_x_assum(fn th => mp_tac th \\ impl_tac >- (strip_tac \\ fs[]) \\ strip_tac)
-      \\ first_x_assum(fn th => mp_tac th \\ impl_tac >- (strip_tac \\ fs[]) \\ strip_tac)
-      \\ first_x_assum(fn th => mp_tac th \\ impl_tac >- (every_case_tac \\ fs[]) \\ strip_tac)
-      \\ first_x_assum(qspec_then`k'`mp_tac) \\ fs[]
-      \\ first_x_assum(qspec_then`ck+k`mp_tac) \\ fs[]
-      \\ ntac 2 strip_tac
-      \\ rveq \\ fs[state_component_equality]
-      \\ every_case_tac \\ fs[])
+      \\ dxrule_then drule evaluate_decs_initial_state_clocks
+      \\ rw []
+      \\ every_case_tac \\ fs []
+    )
     \\ fs[eval_sim_def]
     \\ first_x_assum drule
     \\ impl_tac >- (strip_tac \\ fs[])
@@ -758,8 +734,8 @@ Proof
     \\ last_x_assum drule
     \\ impl_keep_tac >- metis_tac []
     \\ strip_tac \\ fs []
-    \\ imp_res_tac evaluate_decs_add_to_clock_initial_state \\ fs []
-    \\ rveq \\ fs []
+    \\ dxrule_then drule evaluate_decs_initial_state_clocks
+    \\ rw []
     \\ every_case_tac \\ fs [])
   \\ DEEP_INTRO_TAC some_intro
   \\ fs [] \\ rw []
@@ -774,10 +750,9 @@ Proof
     \\ impl_keep_tac >- metis_tac []
     \\ strip_tac \\ fs []
     \\ last_x_assum drule
-    \\ imp_res_tac evaluate_decs_add_to_clock_initial_state \\ fs []
-    \\ imp_res_tac evaluate_decs_add_to_clock_initial_state_io_events_mono
-    \\ fs [] \\ rveq
-    \\ every_case_tac \\ fs [] \\ rw [] \\ fs [])
+    \\ dxrule_then drule evaluate_decs_initial_state_clocks
+    \\ rw []
+    \\ every_case_tac \\ fs [])
   \\ qmatch_abbrev_tac `build_lprefix_lub l1 = build_lprefix_lub l2`
   \\ `(lprefix_chain l1 /\ lprefix_chain l2) /\ equiv_lprefix_chain l1 l2`
      suffices_by metis_tac [build_lprefix_lub_thm,
@@ -792,10 +767,12 @@ Proof
     \\ match_mp_tac prefix_chain_lprefix_chain
     \\ simp [prefix_chain_def, PULL_EXISTS]
     \\ qx_genl_tac [`k1`,`k2`]
-    \\ qspecl_then [`k1`,`k2`] mp_tac LESS_EQ_CASES
-    \\ strip_tac \\ fs [LESS_EQ_EXISTS] \\ rveq
-    \\ metis_tac [evaluate_decs_add_to_clock_io_events_mono,
-                  initial_state_with_clock])
+    \\ simp [GSYM miscTheory.FST_pair]
+    \\ rpt (pairarg_tac \\ fs [])
+    \\ dxrule_then drule evaluate_decs_initial_state_clocks
+    \\ rw []
+    \\ simp []
+  )
   \\ simp [equiv_lprefix_chain_thm]
   \\ unabbrev_all_tac \\ simp [PULL_EXISTS]
   \\ simp [LNTH_fromList, PULL_EXISTS, GSYM FORALL_AND_THM]
@@ -813,9 +790,11 @@ Proof
   \\ `ffi1.io_events ≼ t2.ffi.io_events`
      suffices_by (rw [] \\ fs [IS_PREFIX_APPEND] \\ simp [EL_APPEND1])
   \\ qunabbrev_tac `ffi1`
-  \\ metis_tac
-        [evaluate_decs_add_to_clock_io_events_mono,
-         initial_state_with_clock, FST, ADD_SYM]
+  \\ simp [GSYM miscTheory.FST_pair]
+  \\ rpt (pairarg_tac \\ fs [])
+  \\ dxrule_then drule evaluate_decs_initial_state_clocks
+  \\ rw []
+  \\ simp []
 QED
 
 val op_gbag_def = Define `
@@ -919,16 +898,6 @@ Proof
   \\ qid_spec_tac `env`
   \\ qid_spec_tac `funs`
   \\ Induct \\ fs [FORALL_PROD]
-QED
-
-Theorem evaluate_decs_add_to_clock_io_events_mono_alt:
-    evaluate_decs ^s ds = (s1,res) /\
-    evaluate_decs (s with clock := s.clock + extra) ds = (s2,res2) ==>
-    s1.ffi.io_events ≼ s2.ffi.io_events
-Proof
-  rw []
-  \\ assume_tac (SPEC_ALL evaluate_decs_add_to_clock_io_events_mono)
-  \\ rfs []
 QED
 
 (* generic proof support for most val_rel/state_rel examples *)
